Create FunRelation and FunMaps

FunRelation.v
@@ -4,25 +4,25 @@ Require Export
 Require Import
   Coq.Program.Tactics.
 
-Section SetRelation.
+Section FunRelation.
 
 Variable A : Type.
 Variable B : Type.
 
-Record SetRel := mkSetRel {
+Record FunRel := mkFunRel {
   relEns : Ensemble (A * B);
   _      : forall a b b',
              In _ relEns (a, b)  ->
              In _ relEns (a, b') -> b = b'
 }.
 
-Program Definition Empty : SetRel := mkSetRel (Empty_set (A * B)) _.
+Program Definition Empty : FunRel := mkFunRel (Empty_set (A * B)) _.
 Obligation 1. inversion H. Qed.
 
 Program Definition Insert
-        (a : A) (b : B) (r : SetRel)
-        (H : forall b' : B, ~ In _ (relEns r) (a, b')) : SetRel :=
-  mkSetRel (Add _ (relEns r) (a, b)) _.
+        (a : A) (b : B) (r : FunRel)
+        (H : forall b' : B, ~ In _ (relEns r) (a, b')) : FunRel :=
+  mkFunRel (Add _ (relEns r) (a, b)) _.
 Obligation 1.
   destruct r; simpl in *.
   inversion H0; inversion H1; clear H0 H1;
@@ -31,8 +31,8 @@ Obligation 1.
   subst; firstorder.
 Qed.
 
-Program Definition Remove (a : A) (r : SetRel) : SetRel :=
-  mkSetRel (Setminus _ (relEns r) (fun p => fst p = a)) _.
+Program Definition Remove (a : A) (r : FunRel) : FunRel :=
+  mkFunRel (Setminus _ (relEns r) (fun p => fst p = a)) _.
 Obligation 1.
   destruct r; simpl in *.
   inversion H; inversion H0; clear H H0;
@@ -47,7 +47,7 @@ Proof.
   firstorder.
 Qed.
 
-Program Definition Update (a : A) (b : B) (r : SetRel) : SetRel :=
+Program Definition Update (a : A) (b : B) (r : FunRel) : FunRel :=
   Insert a b (Remove a r) _.
 Obligation 1.
   unfold Remove, relEns, Setminus, In.
@@ -55,8 +55,8 @@ Obligation 1.
   firstorder.
 Qed.
 
-Program Definition Move (a a' : A) (r : SetRel) : SetRel :=
-  mkSetRel (fun p => IF fst p = a'
+Program Definition Move (a a' : A) (r : FunRel) : FunRel :=
+  mkFunRel (fun p => IF fst p = a'
                      then relEns r (a, snd p)
                      else relEns (Remove a r) p) _.
 Obligation 1.
@@ -66,12 +66,12 @@ Obligation 1.
   firstorder.
 Qed.
 
-Program Definition Filter (P : A * B -> Prop) (r : SetRel) : SetRel :=
-  mkSetRel (fun p => P p /\ relEns r p) _.
+Program Definition Filter (P : A * B -> Prop) (r : FunRel) : FunRel :=
+  mkFunRel (fun p => P p /\ relEns r p) _.
 Obligation 1. destruct r; simpl in *; firstorder. Qed.
 
-Program Definition Map (f : A * B -> B) (r : SetRel) : SetRel :=
-  mkSetRel (fun p : A * B =>
+Program Definition Map (f : A * B -> B) (r : FunRel) : FunRel :=
+  mkFunRel (fun p : A * B =>
               exists b : B,
                 In _ (relEns r) (fst p, b) /\
                 In _ (Singleton _ (fst p, f (fst p, b))) p) _.
@@ -83,8 +83,8 @@ Obligation 1.
   reflexivity.
 Qed.
 
-Program Definition Modify (a : A) (f : B -> B) (r : SetRel) : SetRel :=
-  mkSetRel (fun p : A * B =>
+Program Definition Modify (a : A) (f : B -> B) (r : FunRel) : FunRel :=
+  mkFunRel (fun p : A * B =>
               IF fst p = a
               then exists b : B,
                 In _ (relEns r) (fst p, b) /\
@@ -98,17 +98,17 @@ Obligation 1.
   reflexivity.
 Qed.
 
-Definition RemoveIf (P : A * B -> Prop) (r : SetRel) : SetRel :=
+Definition RemoveIf (P : A * B -> Prop) (r : FunRel) : FunRel :=
   Filter (fun p => ~ P p) r.
 
-Definition All (P : A * B -> Prop) (r : SetRel) : Prop :=
+Definition All (P : A * B -> Prop) (r : FunRel) : Prop :=
   forall p, In _ (relEns r) p -> P p.
 
-Definition Any (P : A * B -> Prop) (r : SetRel) : Prop :=
+Definition Any (P : A * B -> Prop) (r : FunRel) : Prop :=
   exists p, In _ (relEns r) p -> P p.
 
-Program Definition Define (P : A -> Prop) (b : B) (r : SetRel) : SetRel :=
-  mkSetRel (fun p => IF P (fst p) then snd p = b else relEns r p) _.
+Program Definition Define (P : A -> Prop) (b : B) (r : FunRel) : FunRel :=
+  mkFunRel (fun p => IF P (fst p) then snd p = b else relEns r p) _.
 Obligation 1.
   destruct r; simpl in *.
   unfold In in *; simpl in *.
@@ -117,8 +117,8 @@ Obligation 1.
   reflexivity.
 Qed.
 
-Program Definition Transfer (P : A -> option A) (r r' : SetRel) : SetRel :=
-  mkSetRel (fun p => forall a,
+Program Definition Transfer (P : A -> option A) (r r' : FunRel) : FunRel :=
+  mkFunRel (fun p => forall a,
               IF P a = Some (fst p)
               then relEns r (a, snd p)
               else relEns r' p) _.
@@ -133,7 +133,7 @@ Obligation 1.
   firstorder.
 Qed.
 
-Definition Lookup (a : A) (b : B) (r : SetRel) := In _ (relEns r) (a, b).
+Definition Lookup (a : A) (b : B) (r : FunRel) := In _ (relEns r) (a, b).
 
 Lemma All_Lookup : forall P r, All P r -> forall a b, Lookup a b r -> P (a, b).
 Proof.
@@ -141,15 +141,15 @@ Proof.
   firstorder.
 Qed.
 
-Lemma Lookup_Remove : forall a b a' r,
+Lemma Lookup_Remove_inv : forall a b a' r,
   Lookup a b (Remove a' r) -> a <> a' /\ Lookup a b r.
 Proof. firstorder. Qed.
 
-Lemma Lookup_Remove_impl : forall a b a' r,
+Lemma Lookup_Remove : forall a b a' r,
   Lookup a b r -> a <> a' -> Lookup a b (Remove a' r).
 Proof. firstorder. Qed.
 
-Lemma Lookup_Update : forall a b a' b' r,
+Lemma Lookup_Update_inv : forall a b a' b' r,
   Lookup a b (Update a' b' r)
     -> IF a = a' then b = b' else Lookup a b r.
 Proof.
@@ -160,14 +160,14 @@ Proof.
   firstorder.
 Qed.
 
-Lemma Lookup_Move : forall a b a' a'' r,
+Lemma Lookup_Move_inv : forall a b a' a'' r,
   Lookup a b (Move a' a'' r)
     -> IF a = a''
        then Lookup a' b r
        else a <> a' /\ Lookup a b r.
 Proof. firstorder. Qed.
 
-Lemma Lookup_Map : forall a b f r,
+Lemma Lookup_Map_inv : forall a b f r,
   Lookup a b (Map f r)
     -> exists b', f (a, b') = b /\ Lookup a b' r.
 Proof.
@@ -178,7 +178,11 @@ Proof.
   firstorder.
 Qed.
 
-Lemma Lookup_Modify : forall a b a' f r,
+Lemma Lookup_Map : forall a b f r,
+  Lookup a b r -> Lookup a (f (a, b)) (Map f r).
+Proof. firstorder. Qed.
+
+Lemma Lookup_Modify_inv : forall a b a' f r,
   Lookup a b (Modify a' f r)
     -> IF a = a'
        then exists b', f b' = b /\ Lookup a b' r
@@ -196,7 +200,7 @@ Proof.
   right; split; trivial.
 Qed.
 
-Definition Member (a : A) (r : SetRel) := exists b, In _ (relEns r) (a, b).
+Definition Member (a : A) (r : FunRel) := exists b, In _ (relEns r) (a, b).
 
 Lemma Member_Remove (addr : A) mem :
   forall addr', Member addr' mem
@@ -210,15 +214,15 @@ Proof. firstorder. Qed.
 Lemma Lookup_Member : forall a b r, Lookup a b r -> Member a r.
 Proof. firstorder. Qed.
 
-Definition FindA (P : A -> Prop) (b : B) (r : SetRel) :=
+Definition FindA (P : A -> Prop) (b : B) (r : FunRel) :=
   forall a, Lookup a b r /\ P a.
 
-Definition FindB (P : B -> Prop) (a : A) (r : SetRel) :=
+Definition FindB (P : B -> Prop) (a : A) (r : FunRel) :=
   forall b, Lookup a b r /\ P b.
 
-End SetRelation.
+End FunRelation.
 
-Arguments mkSetRel : default implicits.
+Arguments mkFunRel : default implicits.
 Arguments relEns : default implicits.
 Arguments Empty : default implicits.
 Arguments Insert : default implicits.
@@ -241,11 +245,11 @@ Arguments FindB : default implicits.
 Ltac teardown :=
   repeat
     match goal with
-    | [ H : Lookup _ _ (Modify _ _ _) |- _ ] => apply Lookup_Modify in H
-    | [ H : Lookup _ _ (Update _ _ _) |- _ ] => apply Lookup_Update in H
-    | [ H : Lookup _ _ (Move _ _ _)   |- _ ] => apply Lookup_Move in H
-    | [ H : Lookup _ _ (Map _ _)      |- _ ] => apply Lookup_Map in H
-    | [ H : Lookup _ _ (Remove _ _)   |- _ ] => apply Lookup_Remove in H
+    | [ H : Lookup _ _ (Modify _ _ _) |- _ ] => apply Lookup_Modify_inv in H
+    | [ H : Lookup _ _ (Update _ _ _) |- _ ] => apply Lookup_Update_inv in H
+    | [ H : Lookup _ _ (Move _ _ _)   |- _ ] => apply Lookup_Move_inv in H
+    | [ H : Lookup _ _ (Map _ _)      |- _ ] => apply Lookup_Map_inv in H
+    | [ H : Lookup _ _ (Remove _ _)   |- _ ] => apply Lookup_Remove_inv in H
 
     | [ H : IF _ then _ else _ |- _ ] => destruct H
     | [ H : _ /\ _             |- _ ] => destruct H
