FunMaps.v
@@ -1,0 +1,114 @@
+Require Import
+  Here.FunRelation
+  Here.Nomega
+  Coq.FSets.FMapAVL
+  Coq.FSets.FMapFacts
+  Coq.Structures.OrderedTypeEx.
+
+Module FunMaps (O : OrderedType).
+
+Module M := FMapAVL.Make(O).
+Module P := FMapFacts.Properties M.
+Module F := P.F.
+
+Definition SetMap_AbsR {A B}
+           (or : FunRel M.key A) (nr : M.t B)
+           (AbsR : A -> B -> Prop) : Prop :=
+  forall addr,
+    (forall data,
+       Lookup addr data or
+         -> (exists cdata, M.find addr nr = Some cdata /\ AbsR data cdata)) /\
+    (forall cdata,
+       M.find addr nr = Some cdata
+         -> (exists data, Lookup addr data or /\ AbsR data cdata)).
+
+Lemma Empty_SetMap_AbsR : forall A B R,
+  SetMap_AbsR (Empty M.key A) (M.empty B) R.
+Proof.
+  split; intros.
+    inversion H.
+  apply F.find_mapsto_iff, F.empty_mapsto_iff in H.
+  contradiction.
+Qed.
+
+Section FunMaps_AbsR.
+
+Variables A B : Type.
+Variable R    : A -> B -> Prop.
+Variable or   : FunRel M.key A.
+Variable nr   : M.t B.
+Variable H    : SetMap_AbsR or nr R.
+
+Hypothesis Oeq_eq : forall a b, O.eq a b -> a = b.
+
+Lemma Update_SetMap_AbsR : forall k v v',
+  R v v' -> SetMap_AbsR (Update k v or) (M.add k v' nr) R.
+Proof.
+  split; intros.
+    teardown; subst.
+      exists v'.
+      split; trivial.
+      apply F.find_mapsto_iff, F.add_mapsto_iff.
+      left; auto.
+    destruct (H addr); clear H H4.
+    destruct (H3 _ H2); clear H2 H3.
+    exists x.
+    intuition.
+    apply F.find_mapsto_iff in H2.
+    apply F.find_mapsto_iff, F.add_mapsto_iff.
+    right; split; auto.
+  apply F.find_mapsto_iff, F.add_mapsto_iff in H1.
+  destruct H1; destruct H1; subst.
+    exists v.
+    split; trivial.
+    apply Oeq_eq in H1; subst.
+    right; constructor.
+  destruct (H addr); clear H H3.
+  apply F.find_mapsto_iff in H2.
+  destruct (H4 _ H2); clear H2 H4.
+  exists x.
+  intuition.
+  left; constructor; auto.
+  unfold Ensembles.In; simpl.
+  unfold not; intros.
+  subst; auto.
+Qed.
+
+Lemma Map_SetMap_AbsR : forall f f',
+  (forall i a b, R a b -> R (f (i, a)) (f' i b))
+    -> SetMap_AbsR (Map f or) (M.mapi f' nr) R.
+Proof.
+  split; intros.
+    teardown; subst.
+    destruct (H addr); clear H H3.
+    destruct (H1 _ H2) as [cdata [? ?]]; clear H1 H2.
+    apply F.find_mapsto_iff in H.
+    exists (f' addr cdata).
+    split.
+      rewrite F.mapi_o, <- F.map_o.
+        apply F.find_mapsto_iff.
+        apply F.map_mapsto_iff.
+        exists cdata; tauto.
+      intros.
+      apply Oeq_eq in H1.
+      subst; reflexivity.
+    apply H0; trivial.
+  rewrite F.mapi_o, <- F.map_o in H1.
+    apply F.find_mapsto_iff in H1.
+    apply F.map_mapsto_iff in H1.
+    destruct H1; destruct H1; subst.
+    apply F.find_mapsto_iff in H2.
+    destruct (H addr); clear H H1.
+    destruct (H3 _ H2) as [data [? ?]]; clear H2 H3.
+    exists (f (addr, data)).
+    split.
+      apply Lookup_Map; trivial.
+    apply H0; trivial.
+  intros.
+  apply Oeq_eq in H2.
+  subst; reflexivity.
+Qed.
+
+End FunMaps_AbsR.
+
+End FunMaps.
